lakefile.lean
@@ -3,7 +3,7 @@ open Lake DSL
 
 package lott
 
-require aesop from git "https://github.com/leanprover-community/aesop" @ "v4.14.0"
+require aesop from git "https://github.com/leanprover-community/aesop" @ "v4.17.0"
 
 lean_lib Lott
 
